

$$\textcircled{1} \quad \frac{\partial L}{\partial w_1} = \frac{\partial L}{\partial h_3} f'_3 w_3 f'_1 x \quad \frac{\partial L}{\partial w_2} = \frac{\partial L}{\partial h_3} f'_3 w_4 f'_2 x$$

$$\frac{\partial L}{\partial w_3} = \frac{\partial L}{\partial h_3} f'_3 h_1 \quad \frac{\partial L}{\partial w_4} = \frac{\partial L}{\partial h_3} f'_3 h_2$$

$$\frac{\partial L}{\partial w_4} = \frac{\partial L}{\partial h_3} f'_3 h_2 \quad \frac{\partial L}{\partial b_1} = \frac{\partial L}{\partial h_3} f'_3 w_3 f'_1 \quad \frac{\partial L}{\partial b_2} = \frac{\partial L}{\partial h_3} f'_3 w_4 f'_2$$

$$\frac{\partial L}{\partial b_3} = \frac{\partial L}{\partial h_3} f'_3 \quad \frac{\partial L}{\partial x} = \frac{\partial L}{\partial h_3} f'_3 (w_3 f'_1 w_1 + w_4 f'_2)$$

$$\textcircled{2} \quad 1. \quad x \rightarrow h = 2x + 1$$

$$h \rightarrow h^2$$

$$x^2 + h^2 \rightarrow z^2$$

$$x \rightarrow x^2$$

$$n \rightarrow e^n = 1 + e^{-n} = y = \frac{1}{1 + e^{-n}}$$

$$2. \quad \frac{\partial y}{\partial x} = 2y(1-y)$$

$\textcircled{3} \quad 1.$ MLP without ReLU simplifies to a linear transformation $y = wx$, as a stack of linear layers simplifies

$2.$ A CNN without ReLU reduces to the same linear operation as convolution is a stacking of linear operations

$\textcircled{4}$ We need to normalize the inputs as they differ on the scale they use.

$$\textcircled{5} \quad 1. \quad y \geq 0 = \text{Softplus}(z) \\ y \leq 0 = \text{Softplus}(z) - 1 \\ a \leq y \leq b = a + (b-a) \sigma(z)$$

$\textcircled{6} \quad 1.$ MLP with ReLU is piecewise linear as each layer is linear

$2.$ IDCNN with ReLU is also piecewise linear for the same reason,

its composed of exclusively linear operations.